Sorting/TreeSort.v
@@ -9,3 +9,70 @@ Require Export ListLemmas.
 Definition treeSort
   {A : Type} (cmp : A -> A -> comparison) (l : list A) : list A :=
     BTree_toList (fromList cmp l).
+
+Lemma Sorted_treeSort :
+  forall (A : Type) (cmp : cmp_spec A) (l : list A),
+    Sorted cmpr (treeSort cmp l).
+Proof.
+  unfold treeSort. intros. apply Sorted_BTree_toList, isBST_fromList.
+Qed.
+
+Lemma perm_treeSort :
+  forall (A : Type) (cmp : A -> A -> comparison) (l : list A),
+    perm (treeSort cmp l) l.
+Proof.
+  induction l as [| h t]; intro; cbn.
+    reflexivity. Search count insert.
+    rewrite count_toList. Search count_BTree. count_BTree_insert, <- count_toList, <- IHt. reflexivity.
+Qed.
+
+Lemma Permutation_treeSort_aux :
+  forall (A : LinDec) (x : A) (t : BTree A),
+    Permutation (BTree_toList (BTree_ins x t)) (x :: BTree_toList t).
+Proof.
+  induction t as [| v l r]; cbn.
+    reflexivity.
+    destruct (x <=? v); cbn.
+      rewrite r. cbn. reflexivity.
+      rewrite IHt1. rewrite Permutation_app_comm, perm_swap. cbn.
+        constructor. rewrite Permutation_app_comm, Permutation_middle.
+          reflexivity.
+Qed.
+
+Lemma Permutation_treeSort :
+  forall (A : LinDec) (l : list A),
+    Permutation (treeSort A l) l.
+Proof.
+  induction l as [| h t]; cbn.
+    reflexivity.
+    rewrite Permutation_treeSort_aux. constructor. assumption.
+Qed.
+
+#[refine]
+Instance Sort_treeSort (A : LinDec) : Sort A :=
+{
+    sort := @treeSort A;
+    Sorted_sort := Sorted_treeSort A;
+}.
+Proof.
+  intros. apply perm_Permutation. rewrite <- perm_treeSort. reflexivity.
+Defined.
+
+Lemma treeSort'_spec :
+  @treeSort' = @treeSort.
+Proof.
+  ext A. ext l. unfold treeSort'.
+  rewrite fromList'_spec, BTree_toList'_spec.
+  unfold treeSort. reflexivity.
+Qed.
+
+#[refine]
+Instance Sort_treeSort' (A : LinDec) : Sort A :=
+{
+    sort := @treeSort' A;
+}.
+Proof.
+  all: intros; rewrite treeSort'_spec.
+    apply Sorted_treeSort.
+    apply perm_Permutation. rewrite <- perm_treeSort. reflexivity.
+Defined.
